proof-libs/coq/ssprove/src/Hacspec_Lib_Integers.v
@@ -36,83 +36,80 @@ Open Scope list_scope.
 
 Import choice.Choice.Exports.
 
-(* Definition lift3_both_ {A B C D : choice_type} {L} {I} (f : A -> B -> C -> D) (x : both L I A) (y : both L I B) (z : both L I C) := *)
+(* Definition lift3_both_ {A B C D : choice_type} {L} {I} (f : A -> B -> C -> D) (x : both A) (y : both B) (z : both C) := *)
 (*   bind_both_ x (fun x' => *)
 (*   bind_both_ y (fun y' => *)
 (*   bind_both_ z (fun z' => *)
 (*   ret_both (f x' y' z')))). *)
 
-Equations int_add {L1 L2 (* L3 *) : {fset Location}} {I1 I2 (* I3 *) : Interface} {WS}
-           (x : both L1 I1 (int WS)) (y : both L2 I2 (int WS))
-           (* `{H_loc_incl_x : is_true (fsubset L1 L3)} `{H_opsig_incl_x : is_true (fsubset I1 I3)} *)
-           (* `{H_loc_incl_y : is_true (fsubset L2 L3)} `{H_opsig_incl_y : is_true (fsubset I2 I3)} *) : both (L1 :|: L2) (* L3 *) (I1 :|: I2) (* I3 *) (int WS) :=
+Equations int_add {WS} (x : both (int WS)) (y : both (int WS)) : both (int WS) :=
   int_add := lift2_both (Hacspec_Lib_Pre.int_add).
-  Fail Next Obligation.
+Fail Next Obligation.
 
-  Equations int_sub {L1 L2 (* L3 *) : {fset Location}} {I1 I2 (* I3 *) : Interface} {WS}
-           (x : both L1 I1 (int WS)) (y : both L2 I2 (int WS))
+  Equations int_sub {WS}
+           (x : both (int WS)) (y : both (int WS))
            (* `{H_loc_incl_x : is_true (fsubset L1 L3)} `{H_opsig_incl_x : is_true (fsubset I1 I3)} *)
-           (* `{H_loc_incl_y : is_true (fsubset L2 L3)} `{H_opsig_incl_y : is_true (fsubset I2 I3)} *) : both (L1 :|: L2) (* L3 *) (I1 :|: I2) (* I3 *) (int WS) :=
+           (* `{H_loc_incl_y : is_true (fsubset L2 L3)} `{H_opsig_incl_y : is_true (fsubset I2 I3)} *) : both (int WS) :=
     int_sub := (lift2_both (Hacspec_Lib_Pre.int_sub)).
   Fail Next Obligation.
 
   Equations int_opp {L (* L2 *) : {fset Location}} {I (* I2 *) : Interface} {WS}
-           (x : both L I (int WS))
-           (* `{H_loc_incl_x : is_true (fsubset L L2)} `{H_opsig_incl_x : is_true (fsubset I I2)} *) : both L I (int WS) :=
+           (x : both (int WS))
+           (* `{H_loc_incl_x : is_true (fsubset L L2)} `{H_opsig_incl_x : is_true (fsubset I I2)} *) : both (int WS) :=
     int_opp := (lift1_both (Hacspec_Lib_Pre.int_opp)).
   Fail Next Obligation.
 
-  Equations int_mul {L1 L2 (* L3 *) : {fset Location}} {I1 I2 (* I3 *) : Interface} {WS}
-           (x : both L1 I1 (int WS)) (y : both L2 I2 (int WS))
+  Equations int_mul {WS}
+           (x : both (int WS)) (y : both (int WS))
            (* `{H_loc_incl_x : is_true (fsubset L1 L3)} `{H_opsig_incl_x : is_true (fsubset I1 I3)} *)
-           (* `{H_loc_incl_y : is_true (fsubset L2 L3)} `{H_opsig_incl_y : is_true (fsubset I2 I3)} *) : both (L1 :|: L2) (* L3 *) (I1 :|: I2) (* I3 *) (int WS) :=
+           (* `{H_loc_incl_y : is_true (fsubset L2 L3)} `{H_opsig_incl_y : is_true (fsubset I2 I3)} *) : both (int WS) :=
     int_mul := (lift2_both (Hacspec_Lib_Pre.int_mul)).
   Fail Next Obligation.
 
-  Equations int_div {L1 L2 (* L3 *) : {fset Location}} {I1 I2 (* I3 *) : Interface} {WS}
-           (x : both L1 I1 (int WS)) (y : both L2 I2 (int WS))
+  Equations int_div {WS}
+           (x : both (int WS)) (y : both (int WS))
            (* `{H_loc_incl_x : is_true (fsubset L1 L3)} `{H_opsig_incl_x : is_true (fsubset I1 I3)} *)
-           (* `{H_loc_incl_y : is_true (fsubset L2 L3)} `{H_opsig_incl_y : is_true (fsubset I2 I3)} *) : both (L1 :|: L2) (* L3 *) (I1 :|: I2) (* I3 *) (int WS) :=
+           (* `{H_loc_incl_y : is_true (fsubset L2 L3)} `{H_opsig_incl_y : is_true (fsubset I2 I3)} *) : both (int WS) :=
     int_div := (lift2_both (Hacspec_Lib_Pre.int_div : int _ -> int _ -> int _)).
   Fail Next Obligation.
 
-  Equations int_mod {L1 L2 (* L3 *) : {fset Location}} {I1 I2 (* I3 *) : Interface} {WS}
-           (x : both L1 I1 (int WS)) (y : both L2 I2 (int WS))
+  Equations int_mod {WS}
+           (x : both (int WS)) (y : both (int WS))
            (* `{H_loc_incl_x : is_true (fsubset L1 L3)} `{H_opsig_incl_x : is_true (fsubset I1 I3)} *)
-           (* `{H_loc_incl_y : is_true (fsubset L2 L3)} `{H_opsig_incl_y : is_true (fsubset I2 I3)} *) : both (L1 :|: L2) (* L3 *) (I1 :|: I2) (* I3 *) (int WS) :=
+           (* `{H_loc_incl_y : is_true (fsubset L2 L3)} `{H_opsig_incl_y : is_true (fsubset I2 I3)} *) : both (int WS) :=
     int_mod := (lift2_both (Hacspec_Lib_Pre.int_mod : int _ -> int _ -> int _)).
   Fail Next Obligation.
 
-  Equations int_xor {L1 L2 (* L3 *) : {fset Location}} {I1 I2 (* I3 *) : Interface} {WS}
-           (x : both L1 I1 (int WS)) (y : both L2 I2 (int WS))
+  Equations int_xor {WS}
+           (x : both (int WS)) (y : both (int WS))
            (* `{H_loc_incl_x : is_true (fsubset L1 L3)} `{H_opsig_incl_x : is_true (fsubset I1 I3)} *)
-           (* `{H_loc_incl_y : is_true (fsubset L2 L3)} `{H_opsig_incl_y : is_true (fsubset I2 I3)} *) : both (L1 :|: L2) (* L3 *) (I1 :|: I2) (* I3 *) (int WS) :=
+           (* `{H_loc_incl_y : is_true (fsubset L2 L3)} `{H_opsig_incl_y : is_true (fsubset I2 I3)} *) : both (int WS) :=
     int_xor := (lift2_both (Hacspec_Lib_Pre.int_xor : int _ -> int _ -> int _)).
   Fail Next Obligation.
 
-  Equations int_and {L1 L2 (* L3 *) : {fset Location}} {I1 I2 (* I3 *) : Interface} {WS}
-           (x : both L1 I1 (int WS)) (y : both L2 I2 (int WS))
+  Equations int_and {WS}
+           (x : both (int WS)) (y : both (int WS))
            (* `{H_loc_incl_x : is_true (fsubset L1 L3)} `{H_opsig_incl_x : is_true (fsubset I1 I3)} *)
-           (* `{H_loc_incl_y : is_true (fsubset L2 L3)} `{H_opsig_incl_y : is_true (fsubset I2 I3)} *) : both (L1 :|: L2) (* L3 *) (I1 :|: I2) (* I3 *) (int WS) :=
+           (* `{H_loc_incl_y : is_true (fsubset L2 L3)} `{H_opsig_incl_y : is_true (fsubset I2 I3)} *) : both (int WS) :=
     int_and := (lift2_both (Hacspec_Lib_Pre.int_and : int _ -> int _ -> int _)).
     Fail Next Obligation.
 
-    Equations int_or {L1 L2 (* L3 *) : {fset Location}} {I1 I2 (* I3 *) : Interface} {WS}
-           (x : both L1 I1 (int WS)) (y : both L2 I2 (int WS))
+    Equations int_or {WS}
+           (x : both (int WS)) (y : both (int WS))
            (* `{H_loc_incl_x : is_true (fsubset L1 L3)} `{H_opsig_incl_x : is_true (fsubset I1 I3)} *)
-           (* `{H_loc_incl_y : is_true (fsubset L2 L3)} `{H_opsig_incl_y : is_true (fsubset I2 I3)} *) : both (L1 :|: L2) (* L3 *) (I1 :|: I2) (* I3 *) (int WS) :=
+           (* `{H_loc_incl_y : is_true (fsubset L2 L3)} `{H_opsig_incl_y : is_true (fsubset I2 I3)} *) : both (int WS) :=
     int_or := (lift2_both (Hacspec_Lib_Pre.int_or : int _ -> int _ -> int _)).
   Fail Next Obligation.
 
   Equations int_not {L (* L2 *) : {fset Location}} {I (* I2 *) : Interface} {WS}
-           (x : both L I (int WS))
-           (* `{H_loc_incl_x : is_true (fsubset L1 L2)} `{H_opsig_incl_x : is_true (fsubset I1 I2)} *) : both L I (int WS) :=
+           (x : both (int WS))
+           (* `{H_loc_incl_x : is_true (fsubset L1 L2)} `{H_opsig_incl_x : is_true (fsubset I1 I2)} *) : both (int WS) :=
     int_not := (lift1_both (Hacspec_Lib_Pre.int_not : int _ -> int _)).
   Fail Next Obligation.
 
   Equations cast_int {L (* L2 *) : {fset Location}} {I (* I2 *) : Interface} {WS1 WS2}
-           (x : both L I (int WS1))
-           (* `{H_loc_incl_x : is_true (fsubset L1 L2)} `{H_opsig_incl_x : is_true (fsubset I1 I2)} *) : both L I (int WS2) :=
+           (x : both (int WS1))
+           (* `{H_loc_incl_x : is_true (fsubset L1 L2)} `{H_opsig_incl_x : is_true (fsubset I1 I2)} *) : both (int WS2) :=
     cast_int := (lift1_both (fun (n : int _) => repr _ (unsigned n))).
   Fail Next Obligation.
 (* End IntType. *)
