proof-libs/coq/ssprove/src/Hacspec_Lib_Coercions.v
@@ -42,67 +42,67 @@ Open Scope list_scope.
 From Hacspec Require Import Hacspec_Lib_Natmod.
 
 (**** Integers to arrays *)
-Definition uint32_to_le_bytes (n : int32) : both (fset []) ([interface]) ((nseq_ int8 4)) := ret_both (uint32_to_le_bytes n).
-Definition uint32_to_be_bytes (n : int32) : both (fset []) ([interface]) ((nseq_ int8 4)) := ret_both (uint32_to_be_bytes n).
-Definition uint32_from_le_bytes (n : (nseq_ int8 4)) : both (fset []) ([interface]) ((int32)) := ret_both (uint32_from_le_bytes n).
-Definition uint32_from_be_bytes (n : (nseq_ int8 4)) : both (fset []) ([interface]) ((int32)) := ret_both (uint32_from_be_bytes n).
-Definition uint64_to_le_bytes (n : int64) : both (fset []) ([interface]) ((nseq_ int8 8)) := ret_both (uint64_to_le_bytes n).
-Definition uint64_to_be_bytes (n : int64) : both (fset []) ([interface]) ((nseq_ int8 8)) := ret_both (uint64_to_be_bytes n).
-Definition uint64_from_le_bytes (n : (nseq_ int8 8)) : both (fset []) ([interface]) ((int64)) := ret_both (uint64_from_le_bytes n).
-Definition uint64_from_be_bytes (n : (nseq_ int8 8)) : both (fset []) ([interface]) ((int64)) := ret_both (uint64_from_be_bytes n).
-Definition uint128_to_le_bytes (n : int128) : both (fset []) ([interface]) ((nseq_ int8 16)) := ret_both (uint128_to_le_bytes n).
-Definition uint128_to_be_bytes (n : int128) : both (fset []) ([interface]) ((nseq_ int8 16)) := ret_both (uint128_to_be_bytes n).
-Definition uint128_from_le_bytes (n : (nseq_ int8 16)) : both (fset []) ([interface]) (int128) := ret_both (uint128_from_le_bytes n).
-Definition uint128_from_be_bytes (n : (nseq_ int8 16)) : both (fset []) ([interface]) ((int128)) := ret_both (uint128_from_be_bytes n).
-Definition u32_to_le_bytes (n : int32) : both (fset []) ([interface]) ((nseq_ int8 4)) := ret_both (u32_to_le_bytes n).
-Definition u32_to_be_bytes (n : int32) : both (fset []) ([interface]) ((nseq_ int8 4)) := ret_both (u32_to_be_bytes n).
-Definition u32_from_le_bytes (n : (nseq_ int8 4)) : both (fset []) ([interface]) ((int32)) := ret_both (u32_from_le_bytes n).
-Definition u32_from_be_bytes (n : (nseq_ int8 4)) : both (fset []) ([interface]) ((int32)) := ret_both (u32_from_be_bytes n).
-Definition u64_to_le_bytes (n : int64) : both (fset []) ([interface]) ((nseq_ int8 8)) := ret_both (u64_to_le_bytes n).
-Definition u64_from_le_bytes (n : (nseq_ int8 8)) : both (fset []) ([interface]) ((int64)) := ret_both (u64_from_le_bytes n).
-Definition u128_to_le_bytes (n : int128) : both (fset []) ([interface]) ((nseq_ int8 16)) := ret_both (u128_to_le_bytes n).
-Definition u128_to_be_bytes (n : int128) : both (fset []) ([interface]) ((nseq_ int8 16)) := ret_both (u128_to_be_bytes n).
-Definition u128_from_le_bytes (n : (nseq_ int8 16)) : both (fset []) ([interface]) ((int128)) := ret_both (u128_from_le_bytes n).
-Definition u128_from_be_bytes (n : (nseq_ int8 16)) : both (fset []) ([interface]) ((int128)) := ret_both (u128_from_be_bytes n).
+Definition uint32_to_le_bytes (n : int32) : both ((nseq_ int8 4)) := ret_both (uint32_to_le_bytes n).
+Definition uint32_to_be_bytes (n : int32) : both ((nseq_ int8 4)) := ret_both (uint32_to_be_bytes n).
+Definition uint32_from_le_bytes (n : (nseq_ int8 4)) : both ((int32)) := ret_both (uint32_from_le_bytes n).
+Definition uint32_from_be_bytes (n : (nseq_ int8 4)) : both ((int32)) := ret_both (uint32_from_be_bytes n).
+Definition uint64_to_le_bytes (n : int64) : both ((nseq_ int8 8)) := ret_both (uint64_to_le_bytes n).
+Definition uint64_to_be_bytes (n : int64) : both ((nseq_ int8 8)) := ret_both (uint64_to_be_bytes n).
+Definition uint64_from_le_bytes (n : (nseq_ int8 8)) : both ((int64)) := ret_both (uint64_from_le_bytes n).
+Definition uint64_from_be_bytes (n : (nseq_ int8 8)) : both ((int64)) := ret_both (uint64_from_be_bytes n).
+Definition uint128_to_le_bytes (n : int128) : both ((nseq_ int8 16)) := ret_both (uint128_to_le_bytes n).
+Definition uint128_to_be_bytes (n : int128) : both ((nseq_ int8 16)) := ret_both (uint128_to_be_bytes n).
+Definition uint128_from_le_bytes (n : (nseq_ int8 16)) : both (int128) := ret_both (uint128_from_le_bytes n).
+Definition uint128_from_be_bytes (n : (nseq_ int8 16)) : both ((int128)) := ret_both (uint128_from_be_bytes n).
+Definition u32_to_le_bytes (n : int32) : both ((nseq_ int8 4)) := ret_both (u32_to_le_bytes n).
+Definition u32_to_be_bytes (n : int32) : both ((nseq_ int8 4)) := ret_both (u32_to_be_bytes n).
+Definition u32_from_le_bytes (n : (nseq_ int8 4)) : both ((int32)) := ret_both (u32_from_le_bytes n).
+Definition u32_from_be_bytes (n : (nseq_ int8 4)) : both ((int32)) := ret_both (u32_from_be_bytes n).
+Definition u64_to_le_bytes (n : int64) : both ((nseq_ int8 8)) := ret_both (u64_to_le_bytes n).
+Definition u64_from_le_bytes (n : (nseq_ int8 8)) : both ((int64)) := ret_both (u64_from_le_bytes n).
+Definition u128_to_le_bytes (n : int128) : both ((nseq_ int8 16)) := ret_both (u128_to_le_bytes n).
+Definition u128_to_be_bytes (n : int128) : both ((nseq_ int8 16)) := ret_both (u128_to_be_bytes n).
+Definition u128_from_le_bytes (n : (nseq_ int8 16)) : both ((int128)) := ret_both (u128_from_le_bytes n).
+Definition u128_from_be_bytes (n : (nseq_ int8 16)) : both ((int128)) := ret_both (u128_from_be_bytes n).
 
 (*** Casting *)
 
 Section TodoSection2.
 
-Definition uint128_from_usize (n : uint_size) : both (fset []) ([interface]) int128 := ret_both (repr _ (unsigned n)).
-Definition uint64_from_usize (n : uint_size) : both (fset []) ([interface]) int64 := ret_both (repr _ (unsigned n)).
-Definition uint32_from_usize (n : uint_size) : both (fset []) ([interface]) int32 := ret_both (repr _ (unsigned n)).
-Definition uint16_from_usize (n : uint_size) : both (fset []) ([interface]) int16 := ret_both (repr _ (unsigned n)).
-Definition uint8_from_usize (n : uint_size) : both (fset []) ([interface]) int8 := ret_both (repr _ (unsigned n)).
+Definition uint128_from_usize (n : uint_size) : both int128 := ret_both (repr _ (unsigned n)).
+Definition uint64_from_usize (n : uint_size) : both int64 := ret_both (repr _ (unsigned n)).
+Definition uint32_from_usize (n : uint_size) : both int32 := ret_both (repr _ (unsigned n)).
+Definition uint16_from_usize (n : uint_size) : both int16 := ret_both (repr _ (unsigned n)).
+Definition uint8_from_usize (n : uint_size) : both int8 := ret_both (repr _ (unsigned n)).
 
-Definition uint128_from_uint8 (n : int8) : both (fset []) ([interface]) int128 := ret_both (repr _ (unsigned n)).
-Definition uint64_from_uint8 (n : int8) : both (fset []) ([interface]) int64 := ret_both (repr _ (unsigned n)).
-Definition uint32_from_uint8 (n : int8) : both (fset []) ([interface]) int32 := ret_both (repr _ (unsigned n)).
-Definition uint16_from_uint8 (n : int8) : both (fset []) ([interface]) int16 := ret_both (repr _ (unsigned n)).
-Definition usize_from_uint8 (n : int8) : both (fset []) ([interface]) uint_size := ret_both (repr _ (unsigned n)).
+Definition uint128_from_uint8 (n : int8) : both int128 := ret_both (repr _ (unsigned n)).
+Definition uint64_from_uint8 (n : int8) : both int64 := ret_both (repr _ (unsigned n)).
+Definition uint32_from_uint8 (n : int8) : both int32 := ret_both (repr _ (unsigned n)).
+Definition uint16_from_uint8 (n : int8) : both int16 := ret_both (repr _ (unsigned n)).
+Definition usize_from_uint8 (n : int8) : both uint_size := ret_both (repr _ (unsigned n)).
 
-Definition uint128_from_uint16 (n : int16) : both (fset []) ([interface]) int128 := ret_both (repr _ (unsigned n)).
-Definition uint64_from_uint16 (n : int16) : both (fset []) ([interface]) int64 := ret_both (repr _ (unsigned n)).
-Definition uint32_from_uint16 (n : int16) : both (fset []) ([interface]) int32 := ret_both (repr _ (unsigned n)).
-Definition uint8_from_uint16 (n : int16) : both (fset []) ([interface]) int8 := ret_both (repr _ (unsigned n)).
-Definition usize_from_uint16 (n : int16) : both (fset []) ([interface]) uint_size := ret_both (repr _ (unsigned n)).
+Definition uint128_from_uint16 (n : int16) : both int128 := ret_both (repr _ (unsigned n)).
+Definition uint64_from_uint16 (n : int16) : both int64 := ret_both (repr _ (unsigned n)).
+Definition uint32_from_uint16 (n : int16) : both int32 := ret_both (repr _ (unsigned n)).
+Definition uint8_from_uint16 (n : int16) : both int8 := ret_both (repr _ (unsigned n)).
+Definition usize_from_uint16 (n : int16) : both uint_size := ret_both (repr _ (unsigned n)).
 
-Definition uint128_from_uint32 (n : int32) : both (fset []) ([interface]) int128 := ret_both (repr _ (unsigned n)).
-Definition uint64_from_uint32 (n : int32) : both (fset []) ([interface]) int64 := ret_both (repr _ (unsigned n)).
-Definition uint16_from_uint32 (n : int32) : both (fset []) ([interface]) int16 := ret_both (repr _ (unsigned n)).
-Definition uint8_from_uint32 (n : int32) : both (fset []) ([interface]) int8 := ret_both (repr _ (unsigned n)).
-Definition usize_from_uint32 (n : int32) : both (fset []) ([interface]) uint_size := ret_both (repr _ (unsigned n)).
+Definition uint128_from_uint32 (n : int32) : both int128 := ret_both (repr _ (unsigned n)).
+Definition uint64_from_uint32 (n : int32) : both int64 := ret_both (repr _ (unsigned n)).
+Definition uint16_from_uint32 (n : int32) : both int16 := ret_both (repr _ (unsigned n)).
+Definition uint8_from_uint32 (n : int32) : both int8 := ret_both (repr _ (unsigned n)).
+Definition usize_from_uint32 (n : int32) : both uint_size := ret_both (repr _ (unsigned n)).
 
-Definition uint128_from_uint64 (n : int64) : both (fset []) ([interface]) int128 := ret_both (repr _ (unsigned n)).
-Definition uint32_from_uint64 (n : int64) : both (fset []) ([interface]) int32 := ret_both (repr _ (unsigned n)).
-Definition uint16_from_uint64 (n : int64) : both (fset []) ([interface]) int16 := ret_both (repr _ (unsigned n)).
-Definition uint8_from_uint64 (n : int64) : both (fset []) ([interface]) int8 := ret_both (repr _ (unsigned n)).
-Definition usize_from_uint64 (n : int64) : both (fset []) ([interface]) uint_size := ret_both (repr _ (unsigned n)).
+Definition uint128_from_uint64 (n : int64) : both int128 := ret_both (repr _ (unsigned n)).
+Definition uint32_from_uint64 (n : int64) : both int32 := ret_both (repr _ (unsigned n)).
+Definition uint16_from_uint64 (n : int64) : both int16 := ret_both (repr _ (unsigned n)).
+Definition uint8_from_uint64 (n : int64) : both int8 := ret_both (repr _ (unsigned n)).
+Definition usize_from_uint64 (n : int64) : both uint_size := ret_both (repr _ (unsigned n)).
 
-Definition uint64_from_uint128 (n : int128) : both (fset []) ([interface]) int64 := ret_both (repr _ (unsigned n)).
-Definition uint32_from_uint128 (n : int128) : both (fset []) ([interface]) int32 := ret_both (repr _ (unsigned n)).
-Definition uint16_from_uint128 (n : int128) : both (fset []) ([interface]) int16 := ret_both (repr _ (unsigned n)).
-Definition uint8_from_uint128 (n : int128) : both (fset []) ([interface]) int8 := ret_both (repr _ (unsigned n)).
-Definition usize_from_uint128 (n : int128) : both (fset []) ([interface]) uint_size := ret_both (repr _ (unsigned n)).
+Definition uint64_from_uint128 (n : int128) : both int64 := ret_both (repr _ (unsigned n)).
+Definition uint32_from_uint128 (n : int128) : both int32 := ret_both (repr _ (unsigned n)).
+Definition uint16_from_uint128 (n : int128) : both int16 := ret_both (repr _ (unsigned n)).
+Definition uint8_from_uint128 (n : int128) : both int8 := ret_both (repr _ (unsigned n)).
+Definition usize_from_uint128 (n : int128) : both uint_size := ret_both (repr _ (unsigned n)).
 
 End TodoSection2.
