proof-libs/coq/ssprove/src/Hacspec_Lib_Natmod.v
@@ -44,26 +44,26 @@ Open Scope list_scope.
 
 Section Todosection.
 
-Definition nat_mod_equal {p} (a b : nat_mod p) : both (fset []) ([interface]) 'bool :=
+Definition nat_mod_equal {p} (a b : nat_mod p) : both 'bool :=
   ret_both (@eqtype.eq_op (fintype_ordinal__canonical__eqtype_Equality (S (Init.Nat.pred (Z.to_nat p)))) a b : 'bool).
 
 Definition nat_mod_equal_reflect {p} {a b} : Bool.reflect (a = b) (is_pure (@nat_mod_equal p a b)) :=
   @eqtype.eqP (fintype_ordinal__canonical__eqtype_Equality (S (Init.Nat.pred (Z.to_nat p)))) a b.
 
-Definition nat_mod_zero {p} : both (fset []) ([interface]) ((nat_mod p)) := ret_both (nat_mod_zero).
-Definition nat_mod_one {p} : both (fset []) ([interface]) ((nat_mod p)) := ret_both (nat_mod_one).
-Definition nat_mod_two {p} : both (fset []) ([interface]) ((nat_mod p)) := ret_both (nat_mod_two).
+Definition nat_mod_zero {p} : both ((nat_mod p)) := ret_both (nat_mod_zero).
+Definition nat_mod_one {p} : both ((nat_mod p)) := ret_both (nat_mod_one).
+Definition nat_mod_two {p} : both ((nat_mod p)) := ret_both (nat_mod_two).
 
-Definition nat_mod_add {n : Z} (a : nat_mod n) (b : nat_mod n) : both (fset []) ([interface]) (nat_mod n) := ret_both (nat_mod_add a b).
-Definition nat_mod_mul {n : Z} (a:nat_mod n) (b:nat_mod n) : both (fset []) ([interface]) (nat_mod n) := ret_both (nat_mod_mul a b).
-Definition nat_mod_sub {n : Z} (a:nat_mod n) (b:nat_mod n) : both (fset []) ([interface]) (nat_mod n) := ret_both (nat_mod_sub a b).
-Definition nat_mod_div {n : Z} (a:nat_mod n) (b:nat_mod n) : both (fset []) ([interface]) (nat_mod n) := ret_both (nat_mod_div a b).
+Definition nat_mod_add {n : Z} (a : nat_mod n) (b : nat_mod n) : both (nat_mod n) := ret_both (nat_mod_add a b).
+Definition nat_mod_mul {n : Z} (a:nat_mod n) (b:nat_mod n) : both (nat_mod n) := ret_both (nat_mod_mul a b).
+Definition nat_mod_sub {n : Z} (a:nat_mod n) (b:nat_mod n) : both (nat_mod n) := ret_both (nat_mod_sub a b).
+Definition nat_mod_div {n : Z} (a:nat_mod n) (b:nat_mod n) : both (nat_mod n) := ret_both (nat_mod_div a b).
 
-Definition nat_mod_neg {n : Z} (a:nat_mod n) : both (fset []) ([interface]) (nat_mod n) := ret_both (nat_mod_neg a).
+Definition nat_mod_neg {n : Z} (a:nat_mod n) : both (nat_mod n) := ret_both (nat_mod_neg a).
 
-Definition nat_mod_inv {n : Z} (a:nat_mod n) : both (fset []) ([interface]) (nat_mod n) := ret_both (nat_mod_inv a).
+Definition nat_mod_inv {n : Z} (a:nat_mod n) : both (nat_mod n) := ret_both (nat_mod_inv a).
 
-Definition nat_mod_exp_def {p : Z} (a:nat_mod p) (n : nat) : both (fset []) ([interface]) (nat_mod p) :=
+Definition nat_mod_exp_def {p : Z} (a:nat_mod p) (n : nat) : both (nat_mod p) :=
   ret_both (nat_mod_exp_def a n).
 
 Definition nat_mod_exp {WS} {p} a n := @nat_mod_exp_def p a (Z.to_nat (@unsigned WS n)).
@@ -73,40 +73,40 @@ Definition nat_mod_pow_self {p} (a n : nat_mod p) := nat_mod_pow_felem a n.
 
 Close Scope nat_scope.
 
-Definition nat_mod_from_secret_literal {m : Z} (x:int128) : both (fset []) ([interface]) (nat_mod m) :=
+Definition nat_mod_from_secret_literal {m : Z} (x:int128) : both (nat_mod m) :=
  ret_both (@nat_mod_from_secret_literal m x).
 
-Definition nat_mod_from_literal (m : Z) (x:int128) : both (fset []) ([interface]) ((nat_mod m)) := nat_mod_from_secret_literal x.
+Definition nat_mod_from_literal (m : Z) (x:int128) : both ((nat_mod m)) := nat_mod_from_secret_literal x.
 
-Definition nat_mod_to_byte_seq_le {n : Z} (m : nat_mod n) : both (fset []) ([interface]) (seq int8) := ret_both (nat_mod_to_byte_seq_le m).
-Definition nat_mod_to_byte_seq_be {n : Z} (m : nat_mod n) : both (fset []) ([interface]) (seq int8) := ret_both (nat_mod_to_byte_seq_be m).
-Definition nat_mod_to_public_byte_seq_le (n : Z) (m : nat_mod n) : both (fset []) ([interface]) (seq int8) := ret_both (nat_mod_to_public_byte_seq_le n m).
-Definition nat_mod_to_public_byte_seq_be (n : Z) (m : nat_mod n) : both (fset []) ([interface]) (seq int8) := ret_both (nat_mod_to_public_byte_seq_be n m).
+Definition nat_mod_to_byte_seq_le {n : Z} (m : nat_mod n) : both (seq int8) := ret_both (nat_mod_to_byte_seq_le m).
+Definition nat_mod_to_byte_seq_be {n : Z} (m : nat_mod n) : both (seq int8) := ret_both (nat_mod_to_byte_seq_be m).
+Definition nat_mod_to_public_byte_seq_le (n : Z) (m : nat_mod n) : both (seq int8) := ret_both (nat_mod_to_public_byte_seq_le n m).
+Definition nat_mod_to_public_byte_seq_be (n : Z) (m : nat_mod n) : both (seq int8) := ret_both (nat_mod_to_public_byte_seq_be n m).
 
-Definition nat_mod_bit {n : Z} (a : nat_mod n) (i : uint_size) : both (fset []) ([interface]) 'bool :=
+Definition nat_mod_bit {n : Z} (a : nat_mod n) (i : uint_size) : both 'bool :=
   ret_both (nat_mod_bit a i).
 
 (* Alias for nat_mod_bit *)
-Definition nat_get_mod_bit {p} (a : nat_mod p) (i : uint_size) : both (fset []) ([interface]) 'bool := ret_both (nat_get_mod_bit a i).
-Definition nat_mod_get_bit {p} (a : nat_mod p) n : both (fset []) ([interface]) (nat_mod p) :=
+Definition nat_get_mod_bit {p} (a : nat_mod p) (i : uint_size) : both 'bool := ret_both (nat_get_mod_bit a i).
+Definition nat_mod_get_bit {p} (a : nat_mod p) n : both (nat_mod p) :=
   ret_both (nat_mod_get_bit a n).
 
-Definition array_declassify_eq {A l} (x : nseq_ A l) (y : nseq_ A l) : both (fset []) ([interface]) 'bool := ret_both (array_declassify_eq x y).
-Definition array_to_le_uint32s {A l} (x : nseq_ A l) : both (fset []) ([interface]) (seq uint32) := ret_both (array_to_le_uint32s x).
-Definition array_to_be_uint32s {l} (x : nseq_ uint8 l) : both (fset []) ([interface]) (seq uint32) := ret_both (array_to_be_uint32s x).
-Definition array_to_le_uint64s {A l} (x : nseq_ A l) : both (fset []) ([interface]) (seq uint64) := ret_both (array_to_le_uint64s x).
-Definition array_to_be_uint64s {l} (x : nseq_ uint8 l) : both (fset []) ([interface]) (seq uint64) := ret_both (array_to_be_uint64s x).
-Definition array_to_le_uint128s {A l} (x : nseq_ A l) : both (fset []) ([interface]) (seq uint128) := ret_both (array_to_le_uint128s x).
-Definition array_to_be_uint128s {l} (x : nseq_ uint8 l) : both (fset []) ([interface]) (seq uint128) := ret_both (array_to_be_uint128s x).
-Definition array_to_le_bytes {A l} (x : nseq_ A l) : both (fset []) ([interface]) (seq uint8) := ret_both (array_to_le_bytes x).
-Definition array_to_be_bytes {A l} (x : nseq_ A l) : both (fset []) ([interface]) (seq uint8) := ret_both (array_to_be_bytes x).
-Definition nat_mod_from_byte_seq_le {A n} (x : seq A) : both (fset []) ([interface]) (nat_mod n) := ret_both (nat_mod_from_byte_seq_le x).
-Definition most_significant_bit {m} (x : nat_mod m) (n : uint_size) : both (fset []) ([interface]) (uint_size) := ret_both (most_significant_bit x n).
+Definition array_declassify_eq {A l} (x : nseq_ A l) (y : nseq_ A l) : both 'bool := ret_both (array_declassify_eq x y).
+Definition array_to_le_uint32s {A l} (x : nseq_ A l) : both (seq uint32) := ret_both (array_to_le_uint32s x).
+Definition array_to_be_uint32s {l} (x : nseq_ uint8 l) : both (seq uint32) := ret_both (array_to_be_uint32s x).
+Definition array_to_le_uint64s {A l} (x : nseq_ A l) : both (seq uint64) := ret_both (array_to_le_uint64s x).
+Definition array_to_be_uint64s {l} (x : nseq_ uint8 l) : both (seq uint64) := ret_both (array_to_be_uint64s x).
+Definition array_to_le_uint128s {A l} (x : nseq_ A l) : both (seq uint128) := ret_both (array_to_le_uint128s x).
+Definition array_to_be_uint128s {l} (x : nseq_ uint8 l) : both (seq uint128) := ret_both (array_to_be_uint128s x).
+Definition array_to_le_bytes {A l} (x : nseq_ A l) : both (seq uint8) := ret_both (array_to_le_bytes x).
+Definition array_to_be_bytes {A l} (x : nseq_ A l) : both (seq uint8) := ret_both (array_to_be_bytes x).
+Definition nat_mod_from_byte_seq_le {A n} (x : seq A) : both (nat_mod n) := ret_both (nat_mod_from_byte_seq_le x).
+Definition most_significant_bit {m} (x : nat_mod m) (n : uint_size) : both (uint_size) := ret_both (most_significant_bit x n).
 
 
 (* We assume 2^x < m *)
 
-Definition nat_mod_pow2 (m : Z) {WS} (x : (@int WS)) : both (fset []) ([interface]) ((nat_mod m)) :=
+Definition nat_mod_pow2 (m : Z) {WS} (x : (@int WS)) : both ((nat_mod m)) :=
   ret_both (nat_mod_pow2 m (Z.to_nat (unsigned x))).
 
 End Todosection.
